\begin{dmath*}
Omega = \frac{1-{{\alppha}}}{1-{{\alppha}}+{{\alppha}}\, {{\epsilon}}}
\end{dmath*}
\begin{dmath*}
psi\_n\_ya = \frac{1+{{\phi}}}{{{\alppha}}+{{\phi}}+\left(1-{{\alppha}}\right)\, {{\sigma}}}
\end{dmath*}
\begin{dmath*}
lambda = \frac{1-{{\alppha}}}{1-{{\alppha}}+{{\alppha}}\, {{\epsilon}}}\, \frac{\left(1-{{\theta}}\right)\, \left(1-{{\theta}}\, {{\beta}}\right)}{{{\theta}}}
\end{dmath*}
\begin{dmath*}
kappa = \left({{\sigma}}+\frac{{{\alppha}}+{{\phi}}}{1-{{\alppha}}}\right)\, \frac{1-{{\alppha}}}{1-{{\alppha}}+{{\alppha}}\, {{\epsilon}}}\, \frac{\left(1-{{\theta}}\right)\, \left(1-{{\theta}}\, {{\beta}}\right)}{{{\theta}}}
\end{dmath*}
% Equation 1
\begin{dmath}
{lam}_{t}={lam\_int}+{rho\_lambda}\, {lam}_{t-1}+{eps\_lambda}_{t}
\end{dmath}
% Equation 2
\begin{dmath}
{Exp\_pi}_{t}={rho}\, {{\pi}}_{t}+\left(1-{rho}\right)\, \left(\left(1-{lam}_{t}\right)\, \left({{\pi}}_{t+1}+{alpha}\right)+{lam}_{t}\, {{\pi}}_{t+1}\right)
\end{dmath}
% Equation 3
\begin{dmath}
{{\pi}}_{t}={{\beta}}\, {Exp\_pi}_{t}+{{\tilde y}}_{t}\, \left({{\sigma}}+\frac{{{\alppha}}+{{\phi}}}{1-{{\alppha}}}\right)\, \frac{1-{{\alppha}}}{1-{{\alppha}}+{{\alppha}}\, {{\epsilon}}}\, \frac{\left(1-{{\theta}}\right)\, \left(1-{{\theta}}\, {{\beta}}\right)}{{{\theta}}}
\end{dmath}
% Equation 4
\begin{dmath}
{{\tilde y}}_{t}=\frac{\left(-1\right)}{{{\sigma}}}\, \left({{i}}_{t}-{Exp\_pi}_{t}-{{r^{nat}}}_{t}\right)+{{\tilde y}}_{t+1}
\end{dmath}
% Equation 5
\begin{dmath}
{Bias}_{t}=\left({Exp\_pi}_{t}-{{\pi}}_{t+1}\right)^{2}
\end{dmath}
% Equation 6
\begin{dmath}
{{r^{nat}}}_{t}=\left({{a}}_{t+1}-{{a}}_{t}\right)\, {{\sigma}}\, \frac{1+{{\phi}}}{{{\alppha}}+{{\phi}}+\left(1-{{\alppha}}\right)\, {{\sigma}}}
\end{dmath}
% Equation 7
\begin{dmath}
{{r^r}}_{t}={{i}}_{t}-{{\pi}}_{t+1}
\end{dmath}
% Equation 8
\begin{dmath}
{{y^{nat}}}_{t}=\frac{1+{{\phi}}}{{{\alppha}}+{{\phi}}+\left(1-{{\alppha}}\right)\, {{\sigma}}}\, {{a}}_{t}
\end{dmath}
% Equation 9
\begin{dmath}
{{\tilde y}}_{t}={{y}}_{t}-{{y^{nat}}}_{t}
\end{dmath}
% Equation 10
\begin{dmath}
{{a}}_{t}={{\rho_a}}\, {{a}}_{t-1}+{{\varepsilon_a}}_{t}
\end{dmath}
% Equation 11
\begin{dmath}
{{y}}_{t}={{a}}_{t}+\left(1-{{\alppha}}\right)\, {{n}}_{t}
\end{dmath}
% Equation 12
\begin{dmath}
{{\Delta m}}_{t}=4\, \left({{\pi}}_{t}+{{y}}_{t}-{{y}}_{t-1}-{{\eta}}\, \left({{i}}_{t}-{{i}}_{t-1}\right)\right)
\end{dmath}
% Equation 13
\begin{dmath}
{{m-p}}_{t}={{y}}_{t}-{{i}}_{t}\, {{\eta}}
\end{dmath}
% Equation 14
\begin{dmath}
{{\Delta m_q}}_{t}={{\pi}}_{t}+{{m-p}}_{t}-{{m-p}}_{t-1}
\end{dmath}
% Equation 15
\begin{dmath}
{{\Delta m_q}}_{t}={{\rho_{m}}}\, {{\Delta m_q}}_{t-1}+{{\varepsilon_\m}}_{t}
\end{dmath}
% Equation 16
\begin{dmath}
{{i^{ann}}}_{t}={{i}}_{t}\, 4
\end{dmath}
% Equation 17
\begin{dmath}
{{r^{r,ann}}}_{t}={{r^r}}_{t}\, 4
\end{dmath}
% Equation 18
\begin{dmath}
{{r^{nat,ann}}}_{t}={{r^{nat}}}_{t}\, 4
\end{dmath}
% Equation 19
\begin{dmath}
{{\pi^{ann}}}_{t}={{\pi}}_{t}\, 4
\end{dmath}
